Added multiple return variables support

theories/Translations/LustreAstToLustre.v
@@ -18,14 +18,14 @@ end.
 Record common_temp : Set := {
   orig :> Source.node;
   env: Dict.t Target.type;
-  Henv: forall x t, Dict.maps_to x (convert_type t) env <-> In (x, t) (orig.(Source.n_in) ++ orig.(Source.n_out) :: orig.(Source.n_locals));
+  Henv: forall x t, Dict.maps_to x (convert_type t) env <-> In (x, t) (orig.(Source.n_in) ++ orig.(Source.n_out) ++ orig.(Source.n_locals));
   
   n_in: list Target.binder;
-  n_out: Target.binder;
+  n_out: list Target.binder;
   n_locals: list Target.binder;
   
-  nvars := n_in ++ n_out :: n_locals;
-  Hnvars: nvars = map (fun '(x, t) => (x, convert_type t)) (orig.(Source.n_in) ++ orig.(Source.n_out) :: orig.(Source.n_locals));
+  nvars := n_in ++ n_out ++ n_locals;
+  Hnvars: nvars = map (fun '(x, t) => (x, convert_type t)) (orig.(Source.n_in) ++ orig.(Source.n_out) ++ orig.(Source.n_locals));
 }.
 
 Open Scope string_scope.
@@ -98,7 +98,7 @@ Proof.
 Defined.
 
 Definition check_body (temp: common_temp) (entry: Source.node): Result.t
-  { body : list Target.equation | incl (map (fun '(n, existT _ ty _) => (n, ty)) body) (nvars temp) }.
+  { body : list Target.equation | incl (map Target.equation_dest body) (nvars temp) }.
 Proof.
   destruct entry.
   induction n_body as [ | [ n e ] tl IH ].
@@ -119,7 +119,7 @@ Proof.
 Defined.
 
 Definition n_assigned_vars (body: list Target.equation) :=
-  map (fun '(n, existT _ ty _) => (n, ty)) body.
+  map Target.equation_dest body.
 
 Scheme Equality for list.
 
@@ -149,22 +149,20 @@ Definition list_eq_dec_binder :=
 Definition list_eq_dec_equation :=
   list_eq_dec _ Source.equation_eqb Source.equation_eqb_to_eq Source.equation_eq_to_eqb.
 
-Definition check_assigned_out (temp: common_temp) body: Result.t (In (n_out temp) (n_assigned_vars body)).
+Definition check_assigned_out (temp: common_temp) body: Result.t (incl (n_out temp) (n_assigned_vars body)).
 Proof.
-  exact (match ListDec.In_dec (prod_dec PeanoNat.Nat.eq_dec Target.type_dec) _ _ with
+  exact (match incl_dec (prod_dec PeanoNat.Nat.eq_dec Target.type_dec) _ _ with
     | left h => Result.Ok h
     | right h => Result.Err "The output variable is never assigned"
   end).
 Defined.
 
 Definition n_out_is_not_an_input (temp: common_temp) :
-  Result.t (~ In (fst (n_out temp)) (map fst (n_in temp))).
-Proof.
-  exact (match ListDec.In_dec PeanoNat.Nat.eq_dec _ _ with
-    | left h => Result.Err "The output variable is also an input"
-    | right h => Result.Ok h
-  end).
-Defined.
+  Result.t (Forall (fun b => ~ In (fst b) (map fst (n_in temp))) (n_out temp)) :=
+  match Forall_dec _ (fun b => dec_not (In_dec PeanoNat.Nat.eq_dec (fst b) _)) _ with
+  | right h => Result.Err "The output variable is also an input"
+  | left h => Result.Ok h
+  end.
 
 
 Definition n_inputs_equations (temp: common_temp) body:
@@ -206,39 +204,29 @@ Proof using.
   left; intros []; assumption.
 Defined.
 
-Definition dec_not {P : Prop} : {P} + {~P} -> {~P} + {~ ~P} :=
-  fun dec => match dec with left h => right (fun nP => nP h) | right h => left h end.
-
 Import Result.notations.
 
 Lemma check_Henv {entry} :
   let n_in := map (fun '(n, t) => (n, convert_type t)) (Source.n_in entry) in
-  let n_out := (fun '(n, t) => (n, convert_type t)) (Source.n_out entry) in
+  let n_out := map (fun '(n, t) => (n, convert_type t)) (Source.n_out entry) in
   let n_locals := map (fun '(n, t) => (n, convert_type t)) (Source.n_locals entry) in
   Result.t (forall n t,
     Dict.maps_to n (convert_type t)
       (fold_left (fun acc '(n, t) => Dict.add n t acc)
-      (n_in ++ n_out :: n_locals)
+      (n_in ++ n_out ++ n_locals)
       (Dict.empty Target.type)) <->
-    In (n, t) (Source.n_in entry ++ Source.n_out entry :: Source.n_locals entry)).
+    In (n, t) (Source.n_in entry ++ Source.n_out entry ++ Source.n_locals entry)).
 Proof using.
-  destruct entry as [? nin [nout tout] nloc ?]; cbn; clear.
-  destruct (In_dec PeanoNat.Nat.eq_dec nout (map fst nin)) as [_|outnotin].
-  1: right; exact "The output variable is in the input list".
-  destruct (In_dec PeanoNat.Nat.eq_dec nout (map fst nloc)) as [_|outnotloc].
-  1: right; exact "The output variable is in the locals list".
-  destruct (Forall_Exists_dec (fun vin => ~ In (fst vin) (map fst nloc))
-    (fun vin => dec_not (In_dec PeanoNat.Nat.eq_dec (fst vin) (map fst nloc))) nin) as [innotloc'|_].
-  2: right; exact "An input variable is in the locals list".
+  destruct entry as [? nin nout nloc ?]; cbn; clear.
   destruct (Forall_Exists_dec (* Technically, does not check for duplicates, only variables with same ID but different types *)
-    (fun vin => forall ty', In (fst vin, ty') nin -> ty' = snd vin)
-    (fun vin =>
+    (fun v => forall ty', In (fst v, ty') nin -> ty' = snd v)
+    (fun v =>
       match forall_type_dec
-        (fun ty' => In (fst vin, ty') nin -> ty' = snd vin)
+        (fun ty' => In (fst v, ty') nin -> ty' = snd v)
         ltac:(
           intros ty;
-          destruct (In_dec (prod_dec PeanoNat.Nat.eq_dec Source.type_dec) (fst vin, ty) nin) as [Hin|Hnin]; [|left; intros f; contradiction (Hnin f)];
-          destruct (Source.type_dec ty (snd vin)) as [eqty|nety]; [left; intros _; exact eqty|];
+          destruct (In_dec (prod_dec PeanoNat.Nat.eq_dec Source.type_dec) (fst v, ty) nin) as [Hin|Hnin]; [|left; intros f; contradiction (Hnin f)];
+          destruct (Source.type_dec ty (snd v)) as [eqty|nety]; [left; intros _; exact eqty|];
           right; intros f; exact (nety (f Hin)))
       with
       | left H => left H
@@ -246,9 +234,31 @@ Proof using.
       end)
     nin) as [innotdup'|_].
   2: right; exact "An input variable is present multiple times in the input list".
-  destruct (Forall_Exists_dec (fun vloc => ~ In (fst vloc) (map fst nin))
-    (fun vloc => dec_not (In_dec PeanoNat.Nat.eq_dec (fst vloc) (map fst nin))) nloc) as [locnotin'|_].
-  2: right; exact "A local variable is in the input list".
+  destruct (Forall_Exists_dec (fun v => ~ In (fst v) (map fst nout))
+    (fun v => dec_not (In_dec PeanoNat.Nat.eq_dec (fst v) (map fst nout))) nin) as [innotout'|_].
+  2: right; exact "An input variable is also an output variable".
+  destruct (Forall_Exists_dec (fun v => ~ In (fst v) (map fst nloc))
+    (fun v => dec_not (In_dec PeanoNat.Nat.eq_dec (fst v) (map fst nloc))) nin) as [innotloc'|_].
+  2: right; exact "An input variable is also a local variable".
+  destruct (Forall_Exists_dec (* Technically, does not check for duplicates, only variables with same ID but different types *)
+    (fun v => forall ty', In (fst v, ty') nout -> ty' = snd v)
+    (fun v =>
+      match forall_type_dec
+        (fun ty' => In (fst v, ty') nout -> ty' = snd v)
+        ltac:(
+          intros ty;
+          destruct (In_dec (prod_dec PeanoNat.Nat.eq_dec Source.type_dec) (fst v, ty) nout) as [Hin|Hnin]; [|left; intros f; contradiction (Hnin f)];
+          destruct (Source.type_dec ty (snd v)) as [eqty|nety]; [left; intros _; exact eqty|];
+          right; intros f; exact (nety (f Hin)))
+      with
+      | left H => left H
+      | right H => right (fun f => match H with ex_intro _ ty Hty => Hty (f ty) end)
+      end)
+    nout) as [outnotdup'|_].
+  2: right; exact "An output variable is present multiple times in the output list".
+  destruct (Forall_Exists_dec (fun v => ~ In (fst v) (map fst nloc))
+    (fun v => dec_not (In_dec PeanoNat.Nat.eq_dec (fst v) (map fst nloc))) nout) as [outnotloc'|_].
+  2: right; exact "An output variable is also a local variable".
   destruct (Forall_Exists_dec (* Technically, does not check for duplicates, only variables with same ID but different types *)
     (fun vloc => forall ty', In (fst vloc, ty') nloc -> ty' = snd vloc)
     (fun vloc =>
@@ -268,112 +278,96 @@ Proof using.
   left; intros n t.
   match goal with |- Dict.maps_to _ _ (fold_left ?f ?l ?d) <-> _ =>
   rewrite <-(fold_left_rev_right (fun x y => f y x) l d) end.
-  rewrite (in_rev (nin ++ (nout, tout) :: nloc) (n, t)),
-          !(rev_app_distr _ (_ :: _) : _ = (rev _ ++ [_]) ++ rev _)%list, <-!(app_assoc _ [_] _ : _ ++ _ :: _ = _)%list, <-!map_rev.
-  apply Forall_rev in innotloc', innotdup', locnotin', locnotdup'.
-  rewrite in_rev, <-map_rev in outnotin, outnotloc.
-  specialize (Forall_impl (P := fun vin => ~ In (fst vin) (map fst nloc)) (fun vin => ~ In (fst vin) (map fst (rev nloc)))
-    (fun vin Hnin Hin => Hnin ltac:(cbn in *; rewrite map_rev, <-in_rev in Hin; exact Hin)) innotloc') as innotloc.
-  specialize (Forall_impl (P := fun vin => ~ In (fst vin) (map fst nin)) (fun vin => ~ In (fst vin) (map fst (rev nin)))
-    (fun vin Hnin Hin => Hnin ltac:(cbn in *; rewrite map_rev, <-in_rev in Hin; exact Hin)) locnotin') as locnotin.
-  specialize (Forall_impl
-    (P := fun vin => forall ty', In (fst vin, ty') nin -> ty' = snd vin)
-    (fun vin => forall ty', In (fst vin, ty') (rev nin) -> ty' = snd vin)
-    (fun vin HP ty' Hin => HP ty' (proj2 (in_rev _ _) Hin)) innotdup') as innotdup.
-  specialize (Forall_impl
-    (P := fun vloc => forall ty', In (fst vloc, ty') nloc -> ty' = snd vloc)
-    (fun vloc => forall ty', In (fst vloc, ty') (rev nloc) -> ty' = snd vloc)
-    (fun vloc HP ty' Hin => HP ty' (proj2 (in_rev _ _) Hin)) locnotdup') as locnotdup.
-  remember (rev nin) as l2 eqn:eq2.
+  rewrite (in_rev (nin ++ nout ++ nloc) (n, t)),
+          !rev_app_distr, <-!app_assoc, <-!map_rev.
+  apply Forall_rev in innotdup', innotloc', innotout', outnotloc', outnotdup', locnotdup'.
+  specialize (Forall_impl _ (fun v HP ty' Hin => HP ty' (proj2 (in_rev _ _) Hin)) innotdup') as innotdup.
+  specialize (Forall_impl _ (fun v Hnin Hin => Hnin (proj2 (in_rev _ _) (eq_ind _ _ Hin _ (map_rev _ _)))) innotout') as innotout.
+  specialize (Forall_impl _ (fun v Hnin Hin => Hnin (proj2 (in_rev _ _) (eq_ind _ _ Hin _ (map_rev _ _)))) innotloc') as innotloc.
+  specialize (Forall_impl _ (fun v HP ty' Hin => HP ty' (proj2 (in_rev _ _) Hin)) outnotdup') as outnotdup.
+  specialize (Forall_impl _ (fun v Hnin Hin => Hnin (proj2 (in_rev _ _) (eq_ind _ _ Hin _ (map_rev _ _)))) outnotloc') as outnotloc.
+  specialize (Forall_impl _ (fun v HP ty' Hin => HP ty' (proj2 (in_rev _ _) Hin)) locnotdup') as locnotdup.
+  remember (rev nin) as l3 eqn:eq3.
+  remember (rev nout) as l2 eqn:eq2.
   remember (rev nloc) as l1 eqn:eq1.
-  clear nloc nin eq1 eq2 innotloc' innotdup' locnotin' locnotdup'.
+  clear nin nout nloc eq1 eq2 eq3 innotdup' innotout' innotloc' outnotdup' outnotloc' locnotdup'.
   split.
   - intros H.
+    clear innotout innotloc outnotloc.
     induction l1 as [|(v, t') l1 IH]; swap 1 2.
     1: destruct (PeanoNat.Nat.eq_dec n v) as [<-|Hne]; [left; f_equal; cbn in H; clear - H|].
     1:  unfold Dict.maps_to in H; rewrite Dict.maps_to_last_added in H.
     1:  injection H as H.
     1:  destruct t, t'; try exact eq_refl; discriminate H.
-    1: right; cbn in *; apply Forall_inv in locnotin as H1; apply Forall_inv in locnotdup as H2.
-    1: apply Forall_inv_tail in locnotin, locnotdup.
-    1: refine (IH (fun h => outnotloc (or_intror h)) (Forall_impl _ _ innotloc) locnotin (Forall_impl _ _ locnotdup) _).
-    1:   intros [b tb] Hb Hin; exact (Hb (or_intror Hin)).
+    1: right; cbn in *; apply Forall_inv in locnotdup as H2.
+    1: apply Forall_inv_tail in locnotdup.
+    1: refine (IH (Forall_impl _ _ locnotdup) _).
     1:  intros [b tb] Hb ty Hin; exact (Hb ty (or_intror Hin)).
     1: exact (Dict.maps_to_not_last_added _ _ _ _ _ H Hne).
-    cbn; clear locnotin innotloc locnotdup outnotloc.
-    destruct (PeanoNat.Nat.eq_dec n nout) as [<-|Hne]; [left; f_equal; cbn in H; clear - H|].
-    1: unfold Dict.maps_to in H; rewrite Dict.maps_to_last_added in H.
-    1: injection H as H.
-    1: destruct t, tout; try exact eq_refl; discriminate H.
-    right; cbn in *.
-    apply Dict.maps_to_not_last_added in H; [|exact Hne].
-    clear nout tout outnotin Hne.
-    induction l2 as [|(v, t') l IH].
-    1: unfold Dict.maps_to, Dict.find, map, fold_right in H.
-    1: rewrite (proj2 (Dict.no_element_is_empty _) eq_refl) in H.
-    1: discriminate H.
-    destruct (PeanoNat.Nat.eq_dec n v) as [<-|Hne]; [left; f_equal; cbn in H; clear - H|].
-    1: unfold Dict.maps_to in H; rewrite Dict.maps_to_last_added in H.
-    1: injection H as H.
-    1: destruct t, t'; try exact eq_refl; discriminate H.
-    right; apply Forall_inv in innotdup as H1.
-    apply Forall_inv_tail in innotdup.
-    refine (IH (Forall_impl _ _ innotdup) _).
-    1: intros [b tb] Hb ty Hin; exact (Hb ty (or_intror Hin)).
-    exact (Dict.maps_to_not_last_added _ _ _ _ _ H Hne).
-  - intros H.
-    induction l1 as [|(v, t') l1 IH]; swap 1 2.
-    1: destruct (prod_dec PeanoNat.Nat.eq_dec Source.type_dec (n, t) (v, t')) as [[=<- <-]|ntnevt'].
-    1:  exact (Dict.maps_to_last_added _ _ _).
-    1: destruct H as [[=-> ->]|H].
-    1:  exact (Dict.maps_to_last_added _ _ _).
-    1: apply Forall_inv in locnotin as H1; apply Forall_inv in locnotdup as H2.
-    1: apply Forall_inv_tail in locnotin, locnotdup.
-    1: refine (Dict.maps_to_add _ _ _ _ _ (IH (fun h => outnotloc (or_intror h)) (Forall_impl _ _ innotloc) locnotin (Forall_impl _ _ locnotdup) H) _).
-    1:   intros [b tb] Hb Hin; exact (Hb (or_intror Hin)).
+    clear locnotdup.
+    induction l2 as [|(v, t') l1 IH]; swap 1 2.
+    1: destruct (PeanoNat.Nat.eq_dec n v) as [<-|Hne]; [left; f_equal; cbn in H; clear - H|].
+    1:  unfold Dict.maps_to in H; rewrite Dict.maps_to_last_added in H.
+    1:  injection H as H.
+    1:  destruct t, t'; try exact eq_refl; discriminate H.
+    1: right; cbn in *; apply Forall_inv in outnotdup as H2.
+    1: apply Forall_inv_tail in outnotdup.
+    1: refine (IH (Forall_impl _ _ outnotdup) _).
     1:  intros [b tb] Hb ty Hin; exact (Hb ty (or_intror Hin)).
-    1: intros <-; refine (ntnevt' (f_equal _ _)); clear IH locnotin H2 ntnevt' innotdup; cbn in *.
-    1: apply in_app_or in H; destruct H as [H|[[=nouteq _]|H]].
-    1:   exact (eq_sym (proj1 (Forall_forall _ _) locnotdup _ H _ (or_introl eq_refl))).
-    1:  contradiction (outnotloc (or_introl (eq_sym nouteq))).
-    1: contradiction (proj1 (Forall_forall _ _) innotloc _ H (or_introl eq_refl)).
-    clear innotloc locnotin locnotdup outnotloc.
-    destruct (prod_dec PeanoNat.Nat.eq_dec Source.type_dec (n, t) (nout, tout)) as [[=<- <-]|Hne].
-    1: exact (Dict.maps_to_last_added _ _ _).
-    destruct H as [[=<- <-]|H].
-    1: exact (Dict.maps_to_last_added _ _ _).
-    cbn; refine (Dict.maps_to_add _ _ _ _ _ _ _); swap 1 2.
-    1: intros <-; refine (Hne (f_equal _ _)); clear Hne; cbn in *.
-    1: contradiction (outnotin (in_map _ _ _ H)).
-    clear nout tout outnotin Hne.
-    induction l2 as [|(v, t') l IH]; [destruct H|].
-    destruct (prod_dec PeanoNat.Nat.eq_dec Source.type_dec (n, t) (v, t')) as [[=<- <-]|ntnevt'].
-    1: exact (Dict.maps_to_last_added _ _ _).
-    destruct H as [[=-> ->]|H].
-    1: exact (Dict.maps_to_last_added _ _ _).
-    apply Forall_inv in innotdup as H2.
-    apply Forall_inv_tail in innotdup.
-    refine (Dict.maps_to_add _ _ _ _ _ (IH (Forall_impl _ _ innotdup) H) _).
-    1: intros [b tb] Hb ty Hin; exact (Hb ty (or_intror Hin)).
-    intros <-; refine (ntnevt' (f_equal _ _)); clear IH H2 ntnevt'; cbn in *.
-    exact (eq_sym (proj1 (Forall_forall _ _) innotdup _ H _ (or_introl eq_refl))).
+    1: exact (Dict.maps_to_not_last_added _ _ _ _ _ H Hne).
+    clear outnotdup.
+    induction l3 as [|(v, t') l1 IH]; swap 1 2.
+    1: destruct (PeanoNat.Nat.eq_dec n v) as [<-|Hne]; [left; f_equal; cbn in H; clear - H|].
+    1:  unfold Dict.maps_to in H; rewrite Dict.maps_to_last_added in H.
+    1:  injection H as H.
+    1:  destruct t, t'; try exact eq_refl; discriminate H.
+    1: right; cbn in *; apply Forall_inv in innotdup as H2.
+    1: apply Forall_inv_tail in innotdup.
+    1: refine (IH (Forall_impl _ _ innotdup) _).
+    1:  intros [b tb] Hb ty Hin; exact (Hb ty (or_intror Hin)).
+    1: exact (Dict.maps_to_not_last_added _ _ _ _ _ H Hne).
+    unfold Dict.maps_to, Dict.find, map, app, fold_right in H.
+    rewrite (proj2 (Dict.no_element_is_empty _) eq_refl) in H.
+    discriminate H.
+  - rewrite !in_app_iff.
+    intros [H|[H|H]].
+    1: rename locnotdup into Hnotdup, l1 into l; clear innotdup outnotdup.
+    2: specialize (proj1 (Forall_forall _ _) outnotloc _ H : ~ In n _) as notinl1.
+    2: rename outnotdup into Hnotdup, l2 into l; clear innotdup locnotdup.
+    3: specialize (proj1 (Forall_forall _ _) innotout _ H : ~ In n _) as notinl2.
+    3: specialize (proj1 (Forall_forall _ _) innotloc _ H : ~ In n _) as notinl1.
+    3: rename innotdup into Hnotdup, l3 into l; clear outnotdup locnotdup.
+    1-3: clear innotout innotloc outnotloc.
+    2-3: induction l1 as [|[n1 t1] l1 IH].
+    2,4: clear notinl1; cbn.
+    4-5: cbn; refine (Dict.maps_to_add _ _ _ _ _ (IH (fun f => notinl1 (or_intror f))) (fun f => notinl1 (or_introl (eq_sym f)))).
+    3: induction l2 as [|[n2 t2] l2 IH].
+    3: clear notinl2; cbn.
+    4: cbn; refine (Dict.maps_to_add _ _ _ _ _ (IH (fun f => notinl2 (or_intror f))) (fun f => notinl2 (or_introl (eq_sym f)))).
+    1-3: induction l as [|[nl tl] l IH]; [contradiction H|].
+    1-3: destruct H as [[=<- <-]|H]; [exact (Dict.maps_to_last_added _ _ _)|].
+    1-3: destruct (PeanoNat.Nat.eq_dec n nl) as [<-|Hne]; [clear IH|].
+    1,3,5: rewrite (proj1 (Forall_forall _ _) Hnotdup _ (or_intror H) _ (or_introl eq_refl)); exact (Dict.maps_to_last_added _ _ _).
+    1-3: refine (Dict.maps_to_add _ _ _ _ _ (IH _ H) Hne).
+    1-3: refine (Forall_impl _ _ (Forall_inv_tail Hnotdup)).
+    1-3: clear; intros x H t Hin; exact (H _ (or_intror Hin)).
 Defined.
 
 Definition check_node_prop (entry: Source.node): Result.t Target.node :=
   let n_in := map (fun '(n, t) => (n, convert_type t)) (Source.n_in entry) in
-  let n_out := (fun '(n, t) => (n, convert_type t)) (Source.n_out entry) in
+  let n_out := map (fun '(n, t) => (n, convert_type t)) (Source.n_out entry) in
   let n_locals := map (fun '(n, t) => (n, convert_type t)) (Source.n_locals entry) in
   do Henv <- check_Henv;
   let temp := {|
     orig := entry;
-    env := fold_left (fun acc '(n, t) => Dict.add n t acc) (n_in ++ n_out :: n_locals) (Dict.empty _);
+    env := fold_left (fun acc '(n, t) => Dict.add n t acc) (n_in ++ n_out ++ n_locals) (Dict.empty _);
     Henv := Henv;
     
     n_in := n_in;
     n_out := n_out;
     n_locals := n_locals;
     
-    Hnvars := eq_sym (map_app _ _ (_ :: _));
+    Hnvars := eq_sym (eq_trans (map_app _ _ _) (f_equal _ (map_app _ _ _)));
   |} in
   do '(exist _ n_body assigned_vars_are_vars) <- check_body temp entry;
   do check_assigned <- check_assigned_out temp n_body;
